formal/SAL-examples/Drinks_Machine_LTL.thy
@@ -1,0 +1,22 @@
+theory Drinks_Machine_LTL
+imports "../examples/Drinks_Machine" EFSM_LTL
+begin
+
+  (* costsMoney: THEOREM drinks |- G(X(cfstate=State_2) => gval(value_ge(r_2, Some(NUM(100))))); *)
+lemma costsMoney: "alw(nxt(StateEq (Some 2)) impl (RegGt 2 100)) (watch drinks i)"
+  oops
+
+(* neverReachS2: THEOREM drinks |- label=select AND I(1) = STR(String_coke) AND
+                                X(label=coin AND I(1) = NUM(100)) AND
+                                X(X(label=vend AND I=InputSequence !empty)) => X(X(X(cfstate=State_2)));;*)
+lemma neverReachS2:"(((((LabelEq ''select'') aand (InputInxEq 1 (Str ''coke'')))
+                    aand
+                    (nxt ((LabelEq ''coin'') aand (InputInxEq 1 (Num 100)))))
+                    aand
+                    (nxt(nxt((LabelEq ''vend'' aand (InputEq []))))))
+                    impl
+                    (nxt(nxt (nxt (StateEq (Some 2))))))
+                    (watch drinks i)"
+  oops
+
+end
